Added lets

Expression.thy
@@ -6,6 +6,7 @@ datatype expr =
   Var nat
 | Abs type expr
 | App expr expr
+| Let expr expr
 | Rec "expr list"
 | Proj expr nat
 | Inj nat "type list" expr
@@ -19,6 +20,7 @@ primrec incr\<^sub>t\<^sub>e :: "nat \<Rightarrow> expr \<Rightarrow> expr" wher
   "incr\<^sub>t\<^sub>e x (Var y) = Var y"
 | "incr\<^sub>t\<^sub>e x (Abs t e) = Abs (incr\<^sub>t\<^sub>t x t) (incr\<^sub>t\<^sub>e x e)"
 | "incr\<^sub>t\<^sub>e x (App e\<^sub>1 e\<^sub>2) = App (incr\<^sub>t\<^sub>e x e\<^sub>1) (incr\<^sub>t\<^sub>e x e\<^sub>2)"
+| "incr\<^sub>t\<^sub>e x (Let e\<^sub>1 e\<^sub>2) = Let (incr\<^sub>t\<^sub>e x e\<^sub>1) (incr\<^sub>t\<^sub>e x e\<^sub>2)"
 | "incr\<^sub>t\<^sub>e x (Rec fs) = Rec (map (incr\<^sub>t\<^sub>e x) fs)"
 | "incr\<^sub>t\<^sub>e x (Proj e l) = Proj (incr\<^sub>t\<^sub>e x e) l"
 | "incr\<^sub>t\<^sub>e x (Inj l ts e) = Inj l (map (incr\<^sub>t\<^sub>t x) ts) (incr\<^sub>t\<^sub>e x e)"
@@ -32,6 +34,7 @@ primrec subst\<^sub>t\<^sub>e :: "nat \<Rightarrow> type \<Rightarrow> expr \<Ri
   "subst\<^sub>t\<^sub>e x t' (Var y) = Var y"
 | "subst\<^sub>t\<^sub>e x t' (Abs t e) = Abs (subst\<^sub>t\<^sub>t x t' t) (subst\<^sub>t\<^sub>e x t' e)"
 | "subst\<^sub>t\<^sub>e x t' (App e\<^sub>1 e\<^sub>2) = App (subst\<^sub>t\<^sub>e x t' e\<^sub>1) (subst\<^sub>t\<^sub>e x t' e\<^sub>2)"
+| "subst\<^sub>t\<^sub>e x t' (Let e\<^sub>1 e\<^sub>2) = Let (subst\<^sub>t\<^sub>e x t' e\<^sub>1) (subst\<^sub>t\<^sub>e x t' e\<^sub>2)"
 | "subst\<^sub>t\<^sub>e x t' (Rec fs) = Rec (map (subst\<^sub>t\<^sub>e x t') fs)"
 | "subst\<^sub>t\<^sub>e x t' (Proj e l) = Proj (subst\<^sub>t\<^sub>e x t' e) l"
 | "subst\<^sub>t\<^sub>e x t' (Inj l ts e) = Inj l (map (subst\<^sub>t\<^sub>t x t') ts) (subst\<^sub>t\<^sub>e x t' e)"
@@ -45,6 +48,7 @@ primrec incr\<^sub>e\<^sub>e :: "nat \<Rightarrow> expr \<Rightarrow> expr" wher
   "incr\<^sub>e\<^sub>e x (Var y) = Var (if x \<le> y then Suc y else y)"
 | "incr\<^sub>e\<^sub>e x (Abs t e) = Abs t (incr\<^sub>e\<^sub>e (Suc x) e)"
 | "incr\<^sub>e\<^sub>e x (App e\<^sub>1 e\<^sub>2) = App (incr\<^sub>e\<^sub>e x e\<^sub>1) (incr\<^sub>e\<^sub>e x e\<^sub>2)"
+| "incr\<^sub>e\<^sub>e x (Let e\<^sub>1 e\<^sub>2) = Let (incr\<^sub>e\<^sub>e x e\<^sub>1) (incr\<^sub>e\<^sub>e (Suc x) e\<^sub>2)"
 | "incr\<^sub>e\<^sub>e x (Rec fs) = Rec (map (incr\<^sub>e\<^sub>e x) fs)"
 | "incr\<^sub>e\<^sub>e x (Proj e l) = Proj (incr\<^sub>e\<^sub>e x e) l"
 | "incr\<^sub>e\<^sub>e x (Inj l ts e) = Inj l ts (incr\<^sub>e\<^sub>e x e)"
@@ -58,6 +62,7 @@ primrec subst\<^sub>e\<^sub>e :: "nat \<Rightarrow> expr \<Rightarrow> expr \<Ri
   "subst\<^sub>e\<^sub>e x e' (Var y) = (if x = y then e' else Var (if x < y then y - 1 else y))"
 | "subst\<^sub>e\<^sub>e x e' (Abs t e) = Abs t (subst\<^sub>e\<^sub>e (Suc x) (incr\<^sub>e\<^sub>e 0 e') e)"
 | "subst\<^sub>e\<^sub>e x e' (App e\<^sub>1 e\<^sub>2) = App (subst\<^sub>e\<^sub>e x e' e\<^sub>1) (subst\<^sub>e\<^sub>e x e' e\<^sub>2)"
+| "subst\<^sub>e\<^sub>e x e' (Let e\<^sub>1 e\<^sub>2) = Let (subst\<^sub>e\<^sub>e x e' e\<^sub>1) (subst\<^sub>e\<^sub>e (Suc x) (incr\<^sub>e\<^sub>e 0 e') e\<^sub>2)"
 | "subst\<^sub>e\<^sub>e x e' (Rec fs) = Rec (map (subst\<^sub>e\<^sub>e x e') fs)"
 | "subst\<^sub>e\<^sub>e x e' (Proj e l) = Proj (subst\<^sub>e\<^sub>e x e' e) l"
 | "subst\<^sub>e\<^sub>e x e' (Inj l ts e) = Inj l ts (subst\<^sub>e\<^sub>e x e' e)"
@@ -72,6 +77,7 @@ primrec is_value :: "expr \<Rightarrow> bool"
   "is_value (Var y) = False"
 | "is_value (Abs t e) = True"
 | "is_value (App e\<^sub>1 e\<^sub>2) = False"
+| "is_value (Let e\<^sub>1 e\<^sub>2) = False"
 | "is_value (Rec fs) = is_value_f fs"
 | "is_value (Proj e l) = False"
 | "is_value (Inj l ts e) = is_value e"
